Add new alpha/rename translation relation and formulate type preservation

src/PlutusIR/Transform/Alpha/Spec.v
@@ -3,65 +3,234 @@ From Coq Require Import
   Lists.List
 .
 From PlutusCert Require Import
+  Util
+  Util.List
   PlutusIR.
 
 Import ListNotations.
 
 Definition ctx := list (string * string).
 
+Reserved Notation "Δ ⊢* s '~' t" (at level 40).
+Reserved Notation "Δ ,, Γ ⊢ s '~' t" (at level 40).
+Reserved Notation "Δ ,, Γ ⊢b s '~' t" (at level 40).
 
-Reserved Notation "Γ ⊢ s '=-α' t" (at level 40).
-Inductive alpha_var : ctx -> string -> string -> Prop :=
-  | AV_refl x : alpha_var [] x x
-  | AV_cons x y xs :
-      alpha_var ((x, y) :: xs) x y
-  | AV_diff x y z w xs :
+Inductive alpha_lookup : ctx -> string -> string -> Prop :=
+
+
+  (* This rule seems unnecessary as long as (x,x) is recorded in the
+   * environment. I guess it makes it possible to define alpha equivalent terms
+   * as those related under the empty environment. The alternative is to define
+   * it for open terms by constructing an identity environment for all free
+   * variables.
+   *)
+  (*
+  | AL_refl x :
+      alpha_lookup [] x x
+  *)
+
+  | AL_cons x y xs :
+      alpha_lookup ((x, y) :: xs) x y
+
+  | AL_diff x y z w xs :
       x <> z ->
       y <> w ->
-      alpha_var xs z w ->
-      alpha_var ((x, y) :: xs) z w
+      alpha_lookup xs z w ->
+      alpha_lookup ((x, y) :: xs) z w
 .
 
-Inductive alpha : list (string * string) -> term -> term -> Prop :=
-  | A_Var x x' xs :
-      alpha_var xs x x' ->
-      xs ⊢ Var x =-α Var x'
-  | A_LamAbs x x' T t t' Γ :
-      ((x, x') :: Γ) ⊢ t =-α t' ->
-      Γ ⊢ LamAbs x T t =-α LamAbs x' T t'
-  | A_Apply t1 t2 t1' t2' Γ :
-      Γ ⊢ t1 =-α t1' ->
-      Γ ⊢ t2 =-α t2' ->
-      Γ ⊢ Apply t1 t2 =-α Apply t1' t2'
 
-  where "Γ ⊢ s '=-α' t" := (alpha Γ s t)
-.
+Module TY.
 
-Section Reflexivity.
+  Inductive ty_alpha : list (string * string) -> ty -> ty -> Prop :=
+
+    | A_TyVar X X' Δ :
+        alpha_lookup Δ X X' ->
+        Δ ⊢* Ty_Var X ~ Ty_Var X'
+
+    | A_TyLam X X' K T T' Δ :
+        ((X, X') :: Δ) ⊢* T ~ T' ->
+        Δ ⊢* Ty_Lam X K T ~ Ty_Lam X' K T'
+
+    | A_TyApp T1 T2 T1' T2' Δ :
+        Δ ⊢* T1 ~ T1' ->
+        Δ ⊢* T2 ~ T2' ->
+        Δ ⊢* Ty_App T1 T2 ~ Ty_App T1' T2'
+
+    | A_TyFun T1 T2 T1' T2' Δ :
+        Δ ⊢* T1 ~ T1' ->
+        Δ ⊢* T2 ~ T2' ->
+        Δ ⊢* Ty_Fun T1 T2 ~ Ty_Fun T1' T2'
+
+    | A_TyIFix T1 T2 T1' T2' Δ :
+        Δ ⊢* T1 ~ T1' ->
+        Δ ⊢* T2 ~ T2' ->
+        Δ ⊢* Ty_IFix T1 T2 ~ Ty_IFix T1' T2'
+
+    | A_TyForall X X' K T T' Δ :
+        ((X, X') :: Δ) ⊢* T ~ T' ->
+        Δ ⊢* Ty_Forall X K T ~ Ty_Forall X' K T'
+
+    | A_TyBuiltin Δ U :
+        Δ ⊢* Ty_Builtin U ~ Ty_Builtin U
+
+    | A_TySOP Δ Tss Tss':
+        ForallSetPair2 (fun T T' => Δ ⊢* T ~ T') Tss Tss' ->
+        Δ ⊢* Ty_SOP Tss ~ Ty_SOP Tss'
+
+    where "Δ ⊢* s '~' t" := (ty_alpha Δ s t)
+  .
+
+
 
   Definition ctx_refl (xs : ctx) := Forall (fun '(x, y) => x = y) xs.
 
   Lemma alpha_refl xs t :
     ctx_refl xs ->
-    alpha xs t t.
+    xs ⊢* t ~ t.
   Proof.
   Admitted.
 
-End Reflexivity.
-
-Section Symmetry.
 
   Inductive pair_sym : string * string -> string * string -> Prop :=
     | PS_pair x y : pair_sym (x, y) (y, x)
   .
+
   Definition ctx_sym (xs ys : ctx) : Prop := Forall2 pair_sym xs ys.
 
   Lemma alpha_sym xs ys t t':
     ctx_sym xs ys ->
-    alpha xs t t' ->
-    alpha ys t' t.
+    xs ⊢* t ~ t' ->
+    ys ⊢* t' ~ t.
   Proof.
   Admitted.
 
-End Symmetry.
+  Inductive pair_trans : string * string -> string * string -> string * string -> Prop :=
+    | PT_pair x y z : pair_trans (x, y) (y, z) (x, z)
+  .
 
+  Definition ctx_trans (xs ys zs : ctx) : Prop := Forall3 pair_trans xs ys zs.
+
+  Lemma alpha_trans xs ys zs t t' t'':
+    ctx_trans xs ys zs ->
+    xs ⊢* t ~ t' ->
+    ys ⊢* t' ~ t'' ->
+    ys ⊢* t ~ t''
+    .
+  Proof.
+  Admitted.
+
+
+End TY.
+
+Import PIRNotations. Open Scope pir_scope.
+Import TY.
+
+Inductive alpha
+  (Δ : list (string * string))
+  (Γ : list (string * string))
+  : term -> term -> Prop :=
+
+  | A_Var x x' :
+      alpha_lookup Γ x x' ->
+      Δ ,, Γ ⊢ `x ~ `x'
+
+  | A_LamAbs x x' T t t' :
+      Δ ,, ((x, x') :: Γ) ⊢ t ~ t' ->
+      Δ ,, Γ ⊢ λ x T t ~ λ x' T t'
+
+  | A_Apply t1 t2 t1' t2' :
+      Δ ,, Γ ⊢ t1 ~ t1' ->
+      Δ ,, Γ ⊢ t2 ~ t2' ->
+      Δ ,, Γ ⊢ (t1 ⋅ t2) ~ (t1' ⋅ t2')
+
+  | A_Let r bs t bs' t' :
+      Δ ,, Γ ⊢ t ~ t' ->
+      Δ ,, Γ ⊢ Let r bs t ~ Let r bs' t'
+
+  | A_TyAbs X K t X' t':
+      ((X, X') :: Δ) ,, Γ ⊢ t ~ t' ->
+      Δ ,, Γ ⊢ (Λ X K t) ~ (Λ X' K t')
+
+  | A_Constant c :
+      Δ ,, Γ ⊢ Constant c ~ Constant c
+
+  | A_Builtin f :
+      Δ ,, Γ ⊢ Builtin f ~ Builtin f
+
+  | A_TyInst t T t' T' :
+      Δ ⊢* T ~ T' ->
+      Δ ,, Γ ⊢ t ~ t' ->
+      Δ ,, Γ ⊢ TyInst t T ~ TyInst t' T'
+
+  | A_Error T T' :
+      Δ ⊢* T ~ T' ->
+      Δ ,, Γ ⊢ Error T ~ Error T'
+
+  | A_IWrap S S' T T' t t' :
+      Δ ⊢* S ~ S' ->
+      Δ ⊢* T ~ T' ->
+      Δ ,, Γ ⊢ t ~ t' ->
+      Δ ,, Γ ⊢ IWrap S T t ~ IWrap S' T' t'
+
+  | A_Unwrap t t' :
+      Δ ,, Γ ⊢ t ~ t' ->
+      Δ ,, Γ ⊢ Unwrap t ~ Unwrap t'
+
+  | A_Constr T i ts T' ts' :
+      Δ ⊢* T ~ T' ->
+      Forall2 (fun t t' => Δ ,, Γ ⊢ t ~ t') ts ts' ->
+      Δ ,, Γ ⊢ Constr T i ts ~ Constr T' i ts'
+
+  | A_Case T t ts T' t' ts' :
+      Δ ⊢* T ~ T' ->
+      Δ ,, Γ ⊢ t ~ t' ->
+      Forall2 (fun t t' => Δ ,, Γ ⊢ t ~ t') ts ts' ->
+      Δ ,, Γ ⊢ Case T t ts ~ Case T' t' ts'
+
+  where "Δ ',,' Γ ⊢ s '~' t" := (alpha Δ Γ s t)
+
+with alpha_binding
+  (Δ : list (string * string))
+  (Γ : list (string * string))
+  : binding -> binding -> Prop :=
+
+  | A_TermBind s x T t x' T' t' :
+    Δ ,, ((x, x') :: Γ) ⊢ t ~ t' ->
+    Δ ,, Γ ⊢b (TermBind s (VarDecl x T) t) ~ (TermBind s (VarDecl x' T') t')
+
+  | A_TypeBind X K T X' T' :
+    ((X, X') :: Δ) ⊢* T ~ T' ->
+    Δ ,, Γ ⊢b (TypeBind (TyVarDecl X K) T) ~ (TypeBind (TyVarDecl X' K) T')
+
+  (* TODO
+  | A_DatatypeBind X K T X' T' :
+    Δ ,, Γ ⊢b  ~
+  *)
+
+  where "Δ ',,' Γ ⊢b b '~' b'" := (alpha_binding Δ Γ b b')
+.
+
+
+Definition ctx_refl (xs : ctx) := Forall (fun '(x, y) => x = y) xs.
+
+Lemma alpha_refl Δ Γ t :
+  ctx_refl Δ ->
+  ctx_refl Γ ->
+  Δ ,, Γ ⊢ t ~ t.
+Proof.
+Admitted.
+
+
+Inductive pair_sym : string * string -> string * string -> Prop :=
+  | PS_pair x y : pair_sym (x, y) (y, x)
+.
+Definition ctx_sym (xs ys : ctx) : Prop := Forall2 pair_sym xs ys.
+
+Lemma alpha_sym Δ Δ' Γ Γ' t t':
+  ctx_sym Δ Δ' ->
+  ctx_sym Γ Γ' ->
+  Δ ,, Γ ⊢ t ~ t' ->
+  Δ' ,, Γ' ⊢ t' ~ t.
+Proof.
+Admitted.
