src/PlutusIR/Semantics/TypeSafety/Preservation.v
@@ -5,6 +5,15 @@ Require Import PlutusCert.PlutusIR.Semantics.TypeSafety.TypeLanguage.Preservatio
 Require Import PlutusCert.PlutusIR.Semantics.Static.Theorems.UniqueTypes.
 Require Import PlutusCert.PlutusIR.Semantics.Static.Theorems.ContextInvariance.AFI.
 
+From PlutusCert Require Import
+  PlutusIR
+  Util.Tactics
+.
+
+Require Import Lists.List.
+Import ListNotations.
+
+
 (* SubstituteT behaves as substituteTCA when substituting closed types *)
 Lemma closed__substituteT_CA :
   forall X U T,
@@ -81,4 +90,120 @@ Proof.
         Decided in meeting April 16 that we will keep it that way and
         will not care about preservation of errors.
         *)
+Admitted.
+
+From PlutusCert Require Import Alpha.Spec.
+
+Import TY.
+
+Axiom ctx_refl_nil : ctx_refl [].
+
+Create HintDb alpha.
+Hint Resolve
+  alpha_refl
+  ctx_refl_nil
+: alpha.
+
+(* shorter syntax for ∃T', ... T' /\ T ~ T' *)
+
+Notation "'∃α' T' '~' T , P" := (exists T' : ty, P /\ [] ⊢* T ~ T')
+  (at level 200, P at level 0, T at level 0, no associativity).
+
+Import PIRNotations.
+Open Scope pir_scope.
+
+Require Import PlutusCert.PlutusIR.Semantics.Static.Typing.Typing.
+(*
+Theorem type_preservation t T v k :
+    t =[k]=> v ->
+    [] ,, [] |-+ t : T ->
+    is_error v \/ (exists T',
+      [] ,, [] |-+ v : T' /\ ty_alpha [] T T').
+      *)
+Theorem type_preservation t T v k :
+    t =[k]=> v ->
+    has_type [] [] t T -> (* TODO, has_type and alpha notation collides *)
+    is_error v \/ ∃α T' ~ T , (has_type [] [] v T').
+Proof with eauto with alpha.
+  intros H_eval.
+  revert T.
+  induction H_eval; intros S H_typing.
+  all: try now (right; exists S; split; eauto with alpha).
+  all: try now (left; constructor). (* Error cases *)
+  - (* Apply *)
+    inversion H_typing; subst.
+
+    repeat match goal with
+    | IH : (forall _, has_type _ _ ?t _ -> _),
+      H_ty : has_type _ _ ?t _ |- _
+      => specialize (IH _ H_ty); clear H_ty
+    end.
+
+    repeat match goal with
+    | IH : (is_error _ \/ _) |- _ =>
+        destruct IH as [H_err | IH];
+        try now inversion H_err
+    end.
+
+    destruct_hypos.
+
+    match goal with
+    | H : has_type [] [] (λ x T t0) x1 |- _ => inversion H; subst
+    end.
+
+    assert (H_ty_subst : (has_type [] [] (subst x v2 t0) T2n))
+      by admit. (* subst preserves typing *)
+
+    specialize (IHH_eval3 T2n H_ty_subst).
+    destruct IHH_eval3; try auto.
+    right.
+    destruct H4 as [T_subst [H_T_subst H_alpha]].
+    eexists.
+    split.
+    eassumption.
+
+    assert (H_S_T2n : [] ⊢* S ~ T2n) by admit. (* Follows from Ty_Fun ~ Ty_Fun ... *)
+
+    eapply alpha_trans.
+    2: eassumption.
+    2: eassumption.
+    constructor.
+  - (* TyInst *)
+    inversion H_typing; subst.
+
+
+    repeat match goal with
+    | IH : (forall _, has_type _ _ ?t _ -> _),
+      H_ty : has_type _ _ ?t _ |- _ => specialize (IH _ H_ty); clear H_ty
+    end.
+    repeat match goal with
+    | IH : (is_error _ \/ _) |- _ =>
+        destruct IH as [H_err | IH];
+        try now inversion H_err
+    end.
+
+    destruct IHH_eval1 as [T_Λ [H_typing_Λ H_alpha_Λ]].
+    inversion H_typing_Λ; subst.
+
+    admit.
+
+  - (* IWrap *)
+    admit.
+  - (* Unwrap *)
+    admit.
+  - (* Built-in Apply *)
+    admit.
+  - (* Built-in TyInst *)
+    admit.
+  - (* Built-in saturated Apply *)
+    admit.
+  - (* Let NonRec *)
+    (* Need IH over eval_bindings_nonrec *)
+    admit.
+  - (* Let Rec *)
+    (* Need IH over eval_bindings_nonrec *)
+    admit.
+  - (* DatatypeBind *)
+    inversion H_typing; subst.
+    admit.
 Admitted.
